src/Examples/Sign/CallString/Example_Sign_DG_CallString_K1.thy
@@ -150,7 +150,7 @@ definition sign_nest_1_eqs ::
   "(pp \<times> cfg_node list, call_string_gk,
      (sign exec_dg_st lifted, sign exec_dg_st lifted) dg_state) eqsT" where
   "sign_nest_1_eqs =
-     routed_node_rhs intra_predecessor_addr_list (\<lambda>_. Global) (cs_route 1)
+     routed_node_rhs intra_predecessor_addr_list call_site_list (\<lambda>_. Global) (cs_route 1)
        (\<lambda>ctx' src a. dg_spec_edge_tree sign_nest_S_st a src (\<lambda>_. Global))
        (routed_call_tree sign_nest_S_st Global Seed (static_resolve sign_nest_cfg)
           (\<lambda>d. d = Bot))
